code/k256/Hacl.Spec.K256.PrecompTable.fst
@@ -5,9 +5,11 @@ open Lib.IntTypes
 open Lib.Sequence
 
 open Hacl.Spec.K256.Field52.Definitions
+open Hacl.Impl.K256.Point
 
 module S = Spec.K256
 module FL = FStar.List.Tot
+module SPT = Hacl.Spec.PrecompBaseTable
 
 #set-options "--z3rlimit 50 --fuel 0 --ifuel 0"
 
@@ -35,46 +37,177 @@ let proj_point_to_list (p:S.proj_point) : point_list =
   [@inline_let] let (px, py, pz) = p in
   FL.(felem_to_list px @ felem_to_list py @ felem_to_list pz)
 
+//----------------------------------------------
+
+let create5_lseq (x0 x1 x2 x3 x4:uint64) : lseq uint64 5 =
+  let l = [x0; x1; x2; x3; x4] in
+  assert_norm (FL.length l = 5);
+  Seq.seq_of_list l
+
+
+val create5_lemma (x0 x1 x2 x3 x4:uint64) :
+  Lemma (let s = create5_lseq x0 x1 x2 x3 x4 in
+    s.[0] == x0 /\ s.[1] == x1 /\ s.[2] == x2 /\ s.[3] == x3 /\ s.[4] == x4)
+let create5_lemma x0 x1 x2 x3 x4 =
+  Seq.elim_of_list [x0; x1; x2; x3; x4]
+
+//-----------------------------------
+
+noextract
+let list_as_felem5 (f:felem_list) : felem5 =
+  let x = Seq.seq_of_list f <: lseq uint64 5 in
+  as_felem5_lseq x
+
+
+val felem_to_list_index_lemma: x:S.felem ->
+  Lemma (let (f0, f1, f2, f3, f4) = list_as_felem5 (felem_to_list x) in
+    let x0 = x % pow52 in
+    let x1 = x / pow52 % pow52 in
+    let x2 = x / pow104 % pow52 in
+    let x3 = x / pow156 % pow52 in
+    let x4 = x / pow208 in
+    v f0 == x0 /\ v f1 == x1 /\ v f2 == x2 /\ v f3 == x3 /\ v f4 == x4)
+
+let felem_to_list_index_lemma x =
+  let x0 = x % pow52 in
+  let x1 = x / pow52 % pow52 in
+  let x2 = x / pow104 % pow52 in
+  let x3 = x / pow156 % pow52 in
+  let x4 = x / pow208 in
+  let f = felem_to_list x in
+
+  let (f0, f1, f2, f3, f4) = list_as_felem5 f in
+  create5_lemma (u64 x0) (u64 x1) (u64 x2) (u64 x3) (u64 x4);
+  assert (v f0 == x0 /\ v f1 == x1 /\ v f2 == x2 /\ v f3 == x3 /\ v f4 == x4)
+
+
+val felem_to_list_lemma_fits: x:S.felem ->
+  Lemma (felem_fits5 (list_as_felem5 (felem_to_list x)) (1, 1, 1, 1, 1))
+
+let felem_to_list_lemma_fits x =
+  felem_to_list_index_lemma x;
+  let x0 = x % pow52 in
+  let x1 = x / pow52 % pow52 in
+  let x2 = x / pow104 % pow52 in
+  let x3 = x / pow156 % pow52 in
+  let x4 = x / pow208 in
+  assert (felem_fits1 (u64 x0) 1);
+  assert (felem_fits1 (u64 x1) 1);
+  assert (felem_fits1 (u64 x2) 1);
+  assert (felem_fits1 (u64 x3) 1);
+  Math.Lemmas.lemma_div_lt_nat x 256 208;
+  assert (felem_fits_last1 (u64 x4) 1)
+
+
+val lemma_mod_pow2_sub: x:nat -> a:nat -> b:nat ->
+  Lemma (x / pow2 a % pow2 b * pow2 a == x % pow2 (a + b) - x % pow2 a)
+
+let lemma_mod_pow2_sub x a b =
+  calc (==) {
+    x / pow2 a % pow2 b * pow2 a;
+    (==) { Math.Lemmas.pow2_modulo_division_lemma_1 x a (a + b) }
+    x % pow2 (a + b) / pow2 a * pow2 a;
+    (==) { Math.Lemmas.euclidean_division_definition (x % pow2 (a + b)) (pow2 a) }
+    x % pow2 (a + b) - x % pow2 (a + b) % pow2 a;
+    (==) { Math.Lemmas.pow2_modulo_modulo_lemma_1 x a (a + b) }
+    x % pow2 (a + b) - x % pow2 a;
+  }
+
+
+val felem_to_list_lemma_eval: x:S.felem ->
+  Lemma (as_nat5 (list_as_felem5 (felem_to_list x)) == x)
+
+let felem_to_list_lemma_eval x =
+  felem_to_list_index_lemma x;
+  let x0 = x % pow52 in
+  let x1 = x / pow52 % pow52 in
+  let x2 = x / pow104 % pow52 in
+  let x3 = x / pow156 % pow52 in
+  let x4 = x / pow208 in
+  let (f0, f1, f2, f3, f4) = list_as_felem5 (felem_to_list x) in
+  let nat_x = as_nat5 (f0, f1, f2, f3, f4) in
+  assert (nat_x == x0 + x1 * pow52 + x2 * pow104 + x3 * pow156 + x4 * pow208);
+  calc (==) {
+    x0 + x1 * pow52 + x2 * pow104 + x3 * pow156 + x4 * pow208;
+    (==) { }
+    x0 + x1 * pow52 + x2 * pow104 + (x / pow156 % pow52) * pow156 + x / pow208 * pow208;
+    (==) { lemma_mod_pow2_sub x 156 52 }
+    x0 + x1 * pow52 + x2 * pow104 + x % pow208 - x % pow156 + x / pow208 * pow208;
+    (==) { Math.Lemmas.euclidean_division_definition x pow208 }
+    x0 + x1 * pow52 + (x / pow104 % pow52) * pow104 - x % pow156 + x;
+    (==) { lemma_mod_pow2_sub x 104 52 }
+    x0 + (x / pow52 % pow52) * pow52 - x % pow104 + x;
+    (==) { lemma_mod_pow2_sub x 52 52 }
+    x;
+  }
+
+//--------------------------------------------
 
 inline_for_extraction noextract
-let g_i_acc_t (i:nat) =
-  S.proj_point & acc:list uint64{FL.length acc == (i + 1) * 15}
+let point_inv_list (p:point_list) =
+  let x = Seq.seq_of_list p <: lseq uint64 15 in
+  point_inv_lseq x
 
-inline_for_extraction noextract
-val precomp_basepoint_table_f (i:nat) (g_i_acc: g_i_acc_t i) : g_i_acc_t (i + 1)
-let precomp_basepoint_table_f i (g_i, acc) =
-  let acc = FL.(acc @ proj_point_to_list g_i) in
-  let g_i = Spec.K256.point_add g_i S.g in
-  g_i, acc
-
-
-// == Loops.repeat_right
-val precomp_basepoint_table_list_rec (n:nat) (acc:g_i_acc_t 0) : Tot (g_i_acc_t n) (decreases n)
-let rec precomp_basepoint_table_list_rec n acc =
-  if n = 0 then acc
-  else precomp_basepoint_table_f (n - 1) (precomp_basepoint_table_list_rec (n - 1) acc)
+noextract
+let point_eval_list (p:point_list) : GTot S.proj_point =
+  let x = Seq.seq_of_list p <: lseq uint64 15 in
+  point_eval_lseq x
 
 
-let precomp_basepoint_table_list_aux : x:list uint64{FL.length x = 240} =
-  snd (precomp_basepoint_table_list_rec 15 (Spec.K256.g, proj_point_to_list S.point_at_inf))
+val proj_point_to_list_sub: p:S.proj_point -> Lemma
+ (let (px, py, pz) = p in
+  let px_list = felem_to_list px in
+  let py_list = felem_to_list py in
+  let pz_list = felem_to_list pz in
+  let p_list = FL.(px_list @ py_list @ pz_list) in
+
+  let p_lseq = Seq.seq_of_list p_list <: lseq uint64 15 in
+  let px_lseq = Seq.seq_of_list px_list <: lseq uint64 5 in
+  let py_lseq = Seq.seq_of_list py_list <: lseq uint64 5 in
+  let pz_lseq = Seq.seq_of_list pz_list <: lseq uint64 5 in
+  sub p_lseq 0 5 == px_lseq /\
+  sub p_lseq 5 5 == py_lseq /\
+  sub p_lseq 10 5 == pz_lseq)
+
+let proj_point_to_list_sub p =
+  let (px, py, pz) = p in
+  let px_list = felem_to_list px in
+  let py_list = felem_to_list py in
+  let pz_list = felem_to_list pz in
+
+  FL.append_assoc px_list py_list pz_list;
+  SPT.seq_of_list_append_lemma px_list py_list;
+  SPT.seq_of_list_append_lemma FL.(px_list @ py_list) pz_list
 
 
-// == Loops.repeat_left
-// val precomp_basepoint_table_list_rec
-//   (n:nat) (i:nat{i <= n}) (acc:g_i_acc_t i) : Tot (g_i_acc_t n) (decreases (n - i))
-// let rec precomp_basepoint_table_list_rec n i acc =
-//   if i = n then acc
-//   else precomp_basepoint_table_list_rec n (i + 1) (precomp_basepoint_table_f i acc)
+val proj_point_to_list_fits: p:S.proj_point ->
+  Lemma (point_inv_list (proj_point_to_list p))
+
+let proj_point_to_list_fits p =
+  let (px, py, pz) = p in
+  proj_point_to_list_sub p;
+  felem_to_list_lemma_fits px;
+  felem_to_list_lemma_fits py;
+  felem_to_list_lemma_fits pz
 
 
-// let precomp_basepoint_table_list_aux : x:list uint64{FL.length x = 240} =
-//   snd (precomp_basepoint_table_list_rec 15 0 (Spec.K256.g, proj_point_to_list S.point_at_inf))
+val proj_point_to_list_eval: p:S.proj_point ->
+  Lemma (point_eval_list (proj_point_to_list p) == p)
+
+let proj_point_to_list_eval p =
+  let (px, py, pz) = p in
+  proj_point_to_list_sub p;
+  felem_to_list_lemma_eval px;
+  felem_to_list_lemma_eval py;
+  felem_to_list_lemma_eval pz;
+  Math.Lemmas.small_mod px S.prime;
+  Math.Lemmas.small_mod py S.prime;
+  Math.Lemmas.small_mod pz S.prime
 
 
-unfold let precomp_basepoint_table_list: x:list uint64{FL.length x = 240} =
-  normalize_term (precomp_basepoint_table_list_aux)
+val proj_point_to_list_lemma: p:S.proj_point ->
+  Lemma (point_inv_list (proj_point_to_list p) /\ point_eval_list (proj_point_to_list p) == p)
 
-
-let precomp_basepoint_table_lseq : lseq uint64 240 =
-  assert_norm (FL.length precomp_basepoint_table_list == 240);
-  Seq.seq_of_list precomp_basepoint_table_list
+let proj_point_to_list_lemma p =
+  proj_point_to_list_fits p;
+  proj_point_to_list_eval p
